theories/proto/proto_enc.v
@@ -5,16 +5,16 @@ Section DualProtoEnc.
   Context `{ValEncDec V} {PROP: bi} .
 
   Definition TSR'
-      (a : action) (P : V → PROP) (prot : V → proto val PROP) : proto val PROP :=
+      (a : action) (Φ : V → PROP) (prot : V → proto val PROP) : proto val PROP :=
     TSR a
-      (λ v, if val_decode v is Some x then P x else False)%I
+      (λ v, if val_decode v is Some x then Φ x else False)%I
       (λ v, if val_decode v is Some x then prot x else TEnd (* dummy *)).
   Global Instance: Params (@TSR') 3.
 
-  Global Instance is_dual_tsr' a1 a2 P (st1 st2 : V → proto val PROP) :
+  Global Instance is_dual_tsr' a1 a2 Φ (st1 st2 : V → proto val PROP) :
     IsDualAction a1 a2 →
     (∀ x, IsDualProto (st1 x) (st2 x)) →
-    IsDualProto (TSR' a1 P st1) (TSR' a2 P st2).
+    IsDualProto (TSR' a1 Φ st1) (TSR' a2 Φ st2).
   Proof.
     rewrite /IsDualAction /IsDualProto. intros <- Hst.
     rewrite -(proto_force_eq (dual_proto _)).
@@ -33,41 +33,39 @@ Notation "<!> x , prot" := (<!> x @ True, (prot x))%proto
   (at level 200, x pattern, prot at level 200) : proto_scope.
 Notation "<?> x , prot" := (<?> x @ True, (prot x))%proto
   (at level 200, x pattern, prot at level 200) : proto_scope.
-Notation "<!> @ P , prot" := (<!> dummy__ @ P dummy__, prot dummy__)%proto
+Notation "<!> @ Φ , prot" := (TSR' Send Φ prot)
   (at level 200, prot at level 200) : proto_scope.
-Notation "<?> @ P , prot" := (<?> dummy__ @ P dummy__, prot dummy__)%proto
+Notation "<?> @ Φ , prot" := (TSR' Receive Φ prot)
   (at level 200, prot at level 200) : proto_scope.
 
 Section proto_enc_specs.
   Context `{!heapG Σ, !logrelG val Σ} `{ValEncDec A} (N : namespace).
 
-  Lemma send_st_spec prot γ c s (P : A → iProp Σ) w :
-    {{{ P w ∗ ⟦ c @ s : <!> @ P, prot ⟧{N,γ} }}}
+  Lemma send_st_spec prot γ c s (Φ : A → iProp Σ) w :
+    {{{ Φ w ∗ ⟦ c @ s : <!> @ Φ, prot ⟧{N,γ} }}}
       send c #s (val_encode w)
     {{{ RET #(); ⟦ c @ s : prot w ⟧{N,γ} }}}.
   Proof.
-    iIntros (Φ) "[HP Hsend] HΦ".
-    iApply (send_st_spec with "[HP $Hsend]").
+    iIntros (Ψ) "[HΦ Hsend] HΨ".
+    iApply (send_st_spec with "[HΦ $Hsend]").
     { by rewrite val_encode_decode. }
     iNext. rewrite val_encode_decode.
-    by iApply "HΦ".
+    by iApply "HΨ".
   Qed.
 
-  Lemma recv_st_spec prot γ c s (P : A → iProp Σ) :
-    {{{ ⟦ c @ s : <?> @ P, prot ⟧{N,γ} }}}
+  Lemma recv_st_spec prot γ c s (Φ : A → iProp Σ) :
+    {{{ ⟦ c @ s : <?> @ Φ, prot ⟧{N,γ} }}}
       recv c #s
-    {{{ v, RET (val_encode v); ⟦ c @ s : prot v ⟧{N,γ} ∗ P v }}}.
+    {{{ v, RET (val_encode v); ⟦ c @ s : prot v ⟧{N,γ} ∗ Φ v }}}.
   Proof.
-    iIntros (Φ) "Hrecv HΦ".
+    iIntros (Ψ) "Hrecv HΨ".
     iApply (recv_st_spec with "Hrecv").
-    iNext. iIntros (v).
-    iIntros "[H HP]".
-    iAssert (∃ w, ⌜val_decode v = Some w⌝ ∗ P w)%I with "[HP]" as (w Hw) "HP".
+    iIntros "!>" (v) "[H HΦ]".
+    iAssert (∃ w, ⌜val_decode v = Some w⌝ ∗ Φ w)%I with "[HΦ]" as (w Hw) "HΦ".
     { destruct (val_decode v) as [x|]; last done.
       iExists x. by iFrame. }
-    iSpecialize ("HΦ" $!w).
     apply val_decode_encode in Hw as <-.
-    iApply "HΦ". iFrame "HP".
+    iApply ("HΨ" $!w). iFrame "HΦ".
     by rewrite val_encode_decode.
   Qed.
 End proto_enc_specs.
